Some massive changes and reog, still in the process to figure out the best implementation

src/main.lean
@@ -1,4 +1,6 @@
 
+notation "⊥" => Empty
+
 inductive Typ : Type
 | base : Typ
 | arrow : Typ → Typ → Typ
@@ -22,21 +24,36 @@ example (A B : Typ ) : (A->B) ≠ A := by
 
 inductive Ctx : Type
 | nil : Ctx 
-| cons : Nat → Ctx → Ctx 
+| cons : Nat → Typ → Ctx → Ctx 
 
 notation "[]" => Ctx.nil
-notation n"⊹"Γ => Ctx.cons n Γ 
+notation n":"t"⊹"Γ => Ctx.cons n t Γ 
 
 namespace Ctx 
 #check []
-#check 4 ⊹ []
-#check 4 ⊹ 3 ⊹ []
+#check 4:base ⊹ []
+#check 4:base ⊹ 3:base ⊹ []
 
-inductive notInCtx : Nat → Ctx → Type 
-| nil : notInCtx n []
-| cons : n₁ ≠ n₂ → notInCtx n₁ Γ → notInCtx n₁ (n₂ ⊹ Γ)   
+inductive inCtx : Nat → Ctx → Type 
+| init : inCtx n (n:A ⊹ Γ) 
+| cons : inCtx n Γ → inCtx n (n₁:A ⊹ Γ)
 
-notation n"¬ε"Γ => notInCtx n Γ
+notation n"ε"Γ => inCtx n Γ
+notation n"¬ε"Γ => inCtx n Γ → False
+
+-- Return a proof that Γ₃ is Γ₁ ++ Γ₂ with no duplicates --
+inductive mergeCtx : Ctx → Ctx → Ctx → Type
+| nil_nil : mergeCtx [] [] []
+| nil_cons : mergeCtx [] Γ Γ 
+| cons_in (n : Nat) (Γ₁ Γ₂ Γ₃ : Ctx) : (n ε Γ₂) → mergeCtx Γ₁ Γ₂ Γ₃ → mergeCtx (n:A ⊹ Γ₁) Γ₂ Γ₃ 
+| cons_out (n : Nat) (Γ₁ Γ₂ Γ₃ : Ctx) : (n ¬ε Γ₂) → mergeCtx Γ₁ Γ₂ Γ₃ → mergeCtx (n:A ⊹ Γ₁) Γ₂ (n:A ⊹ Γ₃) 
+
+inductive validCtx : Ctx → Type 
+| nil : validCtx []
+| cons (n : Nat) (A : Typ) (Γ : Ctx) : (n ¬ε Γ) → validCtx Γ → validCtx (n:A ⊹ Γ)
+notation Γ₃ " ≕ " Γ₁" ⊹ "Γ₂  => mergeCtx Γ₁ Γ₂ Γ₃ 
+
+#check []≕[]⊹[]
 
 inductive Term : Type
 | var : Nat → Term
@@ -44,27 +61,126 @@ inductive Term : Type
 | app : Term → Term → Term
 
 notation "$"n  => Term.var n
-notation n"↦"t => Term.abs n t
-notation t₁"@"t₂ => Term.app t₁ t₂ 
+notation "λ("n")."t => Term.abs n t
+notation "("t₁")("t₂")" => Term.app t₁ t₂ 
 
 namespace Term
 #check $5 
-#check 4 ↦ $5
-#check (4 ↦ $5)@$7
+#check λ(4).$5
+#check (λ(4).$5)($7)
 
 inductive Deduction : Ctx → Term → Typ → Type 
-| var : Deduction (n ⊹ []) ($ n) A
---| weak : (n ¬ε Γ) → Deduction Γ t A → Deduction (n ⊹ Γ) t A 
-| abs : Deduction (n ⊹ Γ) ($ n) A → Deduction Γ t B →  Deduction Γ (n ↦ t) (A->B)
+| var (n : Nat) (A : Typ) : Deduction (n:A ⊹ []) ($ n) A
+| weak (n : Nat) (Γ : Ctx) (A : Typ) : (n ¬ε Γ) → Deduction Γ t A → Deduction (n:B ⊹ Γ) t A 
+| comm (Γ : Ctx) (n₁ n₂ : Nat) (A₁ A₂ : Typ) (t : Term) :
+      Deduction (n₁:A₁ ⊹ n₂:A₂ ⊹ Γ) t A →
+      Deduction (n₂:A₂ ⊹ n₁:A₁ ⊹ Γ) t A
+| abs (n: Nat) (Γ : Ctx) (A B : Typ) : Deduction (n:A ⊹ Γ) ($ n) A → Deduction Γ t B →  Deduction Γ (λ(n).t) (A->B)
+| app (n : Nat) (Γ : Ctx) (t₁ t₂ : Term): Deduction Γ t₁ (A->B) → Deduction Γ t₂ A → Deduction Γ ((t₁)(t₂)) B
 
-notation Γ "⊢" t ":" A => Deduction Γ t A 
+-- WARNING, This is "\:" not just ":" --
+notation Γ " ⊢ " t " ∶ " A => Deduction Γ t A 
 namespace Deduction
 
+theorem ctxSoundness : (Γ ⊢ t ∶ A) → validCtx Γ := by 
+  sorry
+theorem ctxNotNilInDeduction {t : Term} {A : Typ} : ([] ⊢ t ∶ A) → False := by 
+  sorry
+
+theorem noDuplicatesInCtx {n : Nat} {A : Typ} {Γ : Ctx} : validCtx (n:A ⊹ Γ) → n ¬ε Γ := by sorry 
+
+theorem invAbs {n : Nat} {Γ : Ctx} {A B : Typ} {t : Term}: (Γ ⊢ λ(x).t ∶ A->B) → (Γ ⊢ $ x ∶ A) := by 
+  intro h 
+  induction Γ 
+  case nil => 
+    have : False := by exact ctxNotNilInDeduction h  
+    contradiction
+  case cons n A₁ Γ₁ iH => 
+    have : (Γ₁) ⊢ λ(x).t ∶ A->B := by sorry
+    apply Deduction.weak 
+    . intro d 
+      have this2 : validCtx (n:A₁ ⊹ Γ₁) := ctxSoundness h 
+      have this3 : n ¬ε Γ₁  := noDuplicatesInCtx this2 
+      apply this3 
+      exact d
 
 
 
+theorem uniqVar {n n' : Nat} {A : Typ} : ((n:A ⊹ []) ⊢ ($ n') ∶ A) → n = n' := by 
+  intro d  
+  cases d 
+  case var => rfl
+  case weak h d₁ => contradiction 
+    
+
+theorem uniqVarInCtx {n n' : Nat} {Γ : Ctx} {t : Term} {A A' B : Typ} : ((n:A ⊹ n':A' ⊹ Γ) ⊢ t ∶ B) → n ≠ n' := by 
+  intro h 
+  induction t 
+  case var n₁ => 
+    cases h 
+    case weak h' h'' => 
+      intro h₁ 
+      apply h'
+      rw [h₁]
+      apply inCtx.init
+    case comm h' => 
+      intro h₁ 
+      have : validCtx (n':A' ⊹ n:A ⊹ Γ ) := by exact ctxSoundness h' 
+      rw [h₁] at this 
+      cases this 
+      case cons hh hhh=> 
+        apply hhh 
+        apply inCtx.init 
+  case abs n'' t' hh => 
+    apply hh 
+    
+
+  case app => sorry
 
 
+
+example (n₁ n₂ n₃ n₄ : Nat) (A₁ A₂ A₃ A₄ B: Typ) (t : Term) : 
+  ((n₁:A₁  ⊹ n₂:A₂ ⊹ n₃:A₃  ⊹ n₄:A₄  ⊹ []) ⊢ t ∶ B) 
+  → (n₁:A₁  ⊹ n₃:A₃  ⊹ n₂:A₂  ⊹ n₄:A₄  ⊹ []) ⊢ t ∶ B := by 
+  intro d
+  cases t 
+  case var n' => 
+    apply Deduction.weak 
+    case a => 
+      intro d₁ 
+      sorry 
+    case a => sorry
+  case abs => sorry
+  case app => sorry
+
+
+theorem uniqTypForVar (n : Nat) (A B : Typ ) : ((n:A ⊹ []) ⊢ ($ n) ∶ B)→ A = B := by 
+  intros d₂
+  cases d₂ 
+  case var => rfl
+  case weak h d₁ => contradiction
+  
+variable (A B : Typ)
+#check Deduction.var 0 (A->B->A)
+
+--Any term can be constructed no matter the type if we allow free context --
+example {A B : Typ} : Σ Γ : Ctx , Σ t : Term , (Γ ⊢ t ∶ A->B->A) := by
+  let Γ := (0:A->B->A ⊹ [])
+  let t := $0
+  have p : Γ ⊢ t ∶ A->B->A := Deduction.var 0 (A->B->A)
+  exact ⟨ Γ , ⟨ t , p⟩ ⟩ 
+
+-- The story change if we only allow a restricted context, here we need a more intense derivation --
+
+#check 0:base->base ⊹ 1:base ⊹ []
+
+example {A B : Typ} : Σ t : Term , ((0:A->B ⊹ 1:A ⊹ []) ⊢ t ∶ A->B->A) := by
+  constructor
+  case fst => exact λ(1).($0)($1)
+  case snd => 
+    apply Deduction.abs
+    . apply Deduction.weak 
+      
 
 
 
